src/StuartTact.v
@@ -1,3 +1,9 @@
+Require Import List.
+Import ListNotations.
+Require Import Omega.
+Require Import StructTact.StructTactics.
+
+
 Ltac generalize_all :=
     repeat match goal with
     | [ y : _ |- _ ] => generalize y; clear y
@@ -13,9 +19,12 @@ Tactic Notation "make_first" ident(x) :=
 (* Move "x" to the front of the goal, then perform induction. *)
 Ltac first_induction x := make_first x; induction x.
 
+
 Tactic Notation "intros0" ne_ident_list(xs) :=
     intros until 0; intros xs.
 
+
+(* hypothesis pattern matching *)
 
 Tactic Notation "unify" uconstr(x) "with" uconstr(y) :=
     let Htmp := fresh "Htmp" in
@@ -31,6 +40,9 @@ Tactic Notation "on" uconstr(x) "," tactic3(tac) :=
             tac H
     end.
 
+
+(* generic forward reasoning *)
+
 Tactic Notation "fwd" tactic3(tac) "as" ident(H) :=
     simple refine (let H : _ := _ in _);
     [ shelve
@@ -40,6 +52,9 @@ Tactic Notation "fwd" tactic3(tac) "as" ident(H) :=
 Tactic Notation "fwd" tactic3(tac) :=
     let H := fresh "H" in
     fwd tac as H.
+
+
+(* hiding parts of the context *)
 
 Definition sealed {A} (x : A) := x.
 
@@ -52,3 +67,165 @@ Ltac unseal H :=
     match type of H with
     | sealed ?x => change (sealed x) with x in H
     end.
+
+
+(* fun notations *)
+
+Notation "**" := (ltac:(eassumption)) (only parsing).
+Notation "***" := (ltac:(eauto)) (only parsing).
+Notation "??" := (ltac:(shelve)) (only parsing).
+
+
+(* list_magic *)
+
+Lemma Forall_nth_error : forall X (P : X -> Prop) xs,
+    Forall P xs ->
+    (forall i x, nth_error xs i = Some x -> P x).
+intros.
+rewrite Forall_forall in *.
+eauto using nth_error_In.
+Qed.
+
+Lemma nth_error_Forall : forall X (P : X -> Prop) xs,
+    (forall i x, nth_error xs i = Some x -> P x) ->
+    Forall P xs.
+intros. rewrite Forall_forall in *. intros.
+fwd eapply In_nth_error; eauto. break_exists. eauto.
+Qed.
+
+
+Lemma Forall2_length : forall X Y (P : X -> Y -> Prop) xs ys,
+    Forall2 P xs ys ->
+    length xs = length ys.
+induction xs; intros0 Hfa; invc Hfa; simpl; eauto.
+Qed.
+
+Lemma Forall2_nth_error : forall X Y (P : X -> Y -> Prop) xs ys,
+    Forall2 P xs ys ->
+    (forall i x y,
+        nth_error xs i = Some x ->
+        nth_error ys i = Some y ->
+        P x y).
+induction xs; intros0 Hfa; invc Hfa; intros0 Hnx Hny.
+- destruct i; discriminate Hnx.
+- destruct i; simpl in Hnx, Hny.
+  + congruence.
+  + eapply IHxs; eauto.
+Qed.
+
+Lemma nth_error_Forall2 : forall X Y (P : X -> Y -> Prop) xs ys,
+    length xs = length ys ->
+    (forall i x y,
+        nth_error xs i = Some x ->
+        nth_error ys i = Some y ->
+        P x y) ->
+    Forall2 P xs ys.
+induction xs; intros0 Hlen Hnth; destruct ys; invc Hlen.
+- constructor.
+- constructor.
+  + eapply Hnth with (i := 0); reflexivity.
+  + eapply IHxs; eauto.
+    intros. eapply Hnth with (i := S i); simpl; eauto.
+Qed.
+
+Lemma length_nth_error_Some : forall X Y  xs ys x i,
+    @length X xs = @length Y ys ->
+    nth_error xs i = Some x ->
+    exists y, nth_error ys i = Some y.
+intros.
+destruct (nth_error ys i) eqn:?; try eauto.
+rewrite nth_error_None in *.
+assert (nth_error xs i <> None) by congruence.
+rewrite nth_error_Some in *.
+omega.
+Qed.
+
+Lemma Forall2_nth_error_Some : forall X Y (P : X -> Y -> Prop) xs ys x i,
+    Forall2 P xs ys ->
+    nth_error xs i = Some x ->
+    exists y, nth_error ys i = Some y.
+intros. eapply length_nth_error_Some. eapply Forall2_length. all:eauto.
+Qed.
+
+Lemma Forall2_flip : forall A B (P : A -> B -> Prop) (Q : B -> A -> Prop) (xs : list A) (ys : list B),
+    (forall x y, P x y -> Q y x) ->
+    Forall2 P xs ys -> Forall2 Q ys xs.
+induction xs; intros0 Hpq Hfa; invc Hfa; constructor; firstorder eauto.
+Qed.
+
+Lemma Forall2_flip' : forall A B (P : A -> B -> Prop) (xs : list A) (ys : list B),
+    Forall2 P xs ys -> Forall2 (fun y x => P x y) ys xs.
+intros; eapply Forall2_flip; eauto.
+Qed.
+
+
+
+
+Ltac collect_length_hyps :=
+    repeat match goal with
+    | [ H : Forall2 _ ?xs_ ?ys_ |- _ ] =>
+            lazymatch goal with
+            | [ H : length xs_ = length ys_ |- _ ] => idtac (* already known *)
+            | [ |- _ ] => 
+                    fwd eapply Forall2_length with (xs := xs_) (ys := ys_) (1 := H)
+            end
+    end.
+
+Ltac find_matching_entries HH i :=
+    repeat match type of HH with
+    | forall y, nth_error ?ys_ i = Some y -> _ =>
+            first
+                [ specialize (HH ?? **)
+                | let Hexist := fresh "H" in
+                  let y := fresh "y" in
+                  let Hy := fresh "H" y in
+                  fwd eapply length_nth_error_Some with (ys := ys_) as Hexist;
+                  [ | eassumption | ];
+                  [ congruence | ];
+                  destruct Hexist as [y Hy];
+                  specialize (HH y Hy) ]
+    end.
+
+Ltac require_no_match P :=
+    lazymatch goal with
+    | [ H : P |- _ ] => fail "expected no hypothesis matching" P ", but found" H
+    | [ |- _ ] => idtac
+    end.
+
+Ltac collect_entry_hyps i :=
+    repeat match goal with
+    | [ Hfa : Forall ?P ?xs, Hnth : nth_error ?xs i = Some ?x |- _ ] =>
+            require_no_match (P x);
+            assert (P x) by (eapply Forall_nth_error with (1 := Hfa) (2 := Hnth))
+    | [ Hfa : Forall2 ?P ?xs ?ys,
+        Hnx : nth_error ?xs i = Some ?x,
+        Hny : nth_error ?ys i = Some ?y |- _ ] =>
+            require_no_match (P x y);
+            assert (P x y) by
+                (eapply Forall2_nth_error with (1 := Hfa) (2 := Hnx) (3 := Hny))
+    end.
+
+Ltac list_magic HH :=
+    let i := fresh "i" in
+    collect_length_hyps;
+    (eapply nth_error_Forall || (eapply nth_error_Forall2; [congruence | ..]));
+    intro i; intros;
+    specialize (HH i);
+    collect_length_hyps; find_matching_entries HH i; collect_entry_hyps i;
+    eapply HH; eauto.
+
+
+(* hide terms for printing *)
+
+(* Utility tactic for hiding proof terms inside of functions.  This is useful
+   for functions that will sometimes need to be unfolded, to keep the giant
+   proof term from wasting tons of screen space. *)
+
+Definition HIDDEN (A : Type) (x : A) : A := x.
+(* Make all arguments implicit so `@HIDDEN P (giant proof)` prints as `HIDDEN`. *)
+Implicit Arguments HIDDEN [A x].
+
+(* The `hide` tactic wraps (with `HIDDEN`) the remainder of the proof of the
+   current goal.  Use it like `refine (...); hide; prove stuff...` or
+   `$(hide; prove stuff...)$`. *)
+Ltac hide := apply @HIDDEN.
