src/TaggedComp2.v
@@ -1,0 +1,723 @@
+Require Import Common.
+
+Require Import Monads.
+Require Import StuartTact.
+Require Utopia.
+
+Require Lifted.
+Require Tagged.
+
+Module L := Lifted.
+Module T := Tagged.
+
+
+Section compile.
+Open Scope option_monad.
+
+Definition mk_rec_info ctor :=
+    let fix go acc n :=
+        match n with
+        | 0 => acc
+        | S n => go (Utopia.ctor_arg_is_recursive ctor n :: acc) n
+        end in
+    go [] (Utopia.constructor_arg_n ctor).
+
+Fixpoint mk_tagged_cases' ty idx cases : option (list (T.expr * T.rec_info)) :=
+    match cases with
+    | [] => Some []
+    | case :: cases =>
+            Utopia.type_constr ty idx >>= fun ctor =>
+            mk_tagged_cases' ty (S idx) cases >>= fun cases' =>
+            Some ((case, mk_rec_info ctor) :: cases')
+    end.
+
+Definition mk_tagged_cases ty cases :=
+    mk_tagged_cases' ty 0 cases.
+
+Definition compile (e : L.expr) : option T.expr :=
+    let fix go e :=
+        let fix go_list es :=
+            match es with
+            | [] => Some []
+            | e :: es => cons <$> go e <*> go_list es
+            end in
+        match e with
+        | L.Arg => Some (T.Arg)
+        | L.UpVar n => Some (T.UpVar n)
+        | L.Call f a => T.Call <$> go f <*> go a
+        | L.Constr c args => T.Constr (Utopia.constructor_index c) <$> go_list args
+        | L.Elim ty cases target =>
+                go_list cases >>= fun cases =>
+                T.Elim <$> mk_tagged_cases ty cases <*> go target
+        | L.Close f free => T.Close f <$> go_list free
+        end in go e.
+
+Definition compile_list :=
+    let fix go_list (es : list L.expr) : option (list T.expr) :=
+        match es with
+        | [] => Some []
+        | e :: es => cons <$> compile e <*> go_list es
+        end in go_list.
+
+Definition compile_program (lp : L.expr * list L.expr) : option (T.expr * list T.expr) :=
+  pair <$> (compile (fst lp)) <*> compile_list (snd lp).
+
+End compile.
+
+
+(* spec *)
+
+Inductive R (LE : L.env) (TE : T.env) : L.expr -> T.expr -> Prop :=
+| RConstr : forall c largs targs,
+        Forall2 (R LE TE) largs targs ->
+        R LE TE
+            (L.Constr c largs)
+            (T.Constr (Utopia.constructor_index c) targs)
+| RClose : forall fn lf tf lfree tfree,
+        nth_error LE fn = Some lf ->
+        nth_error TE fn = Some tf ->
+        compile_program (lf, LE) = Some (tf, TE) ->
+        Forall2 (R LE TE) lfree tfree ->
+        R LE TE
+            (L.Close fn lfree)
+            (T.Close fn tfree)
+.
+
+Definition R_value_thm := forall LE TE l t,
+    L.value l ->
+    compile_program (l, LE) = Some (t, TE) ->
+    R LE TE l t.
+
+Definition R_call_sim_thm := forall LE TE lf la lr tf ta,
+    R LE TE lf tf ->
+    R LE TE la ta ->
+    L.star LE (L.Call lf la) lr ->
+    exists tr,
+        T.star TE (T.Call tf ta) tr /\
+        R LE TE lr tr.
+
+
+(* inductive relation *)
+
+Inductive I (LE : L.env) (TE : T.env) : L.expr -> T.expr -> Prop :=
+| ICompile : forall l t,
+        compile_list LE = Some TE ->
+        compile l = Some t ->
+        I LE TE l t.
+
+Definition I_R_value_thm := forall LE TE l t,
+    L.value l ->
+    T.value t ->
+    R LE TE l t <-> I LE TE l t.
+
+Definition I_sim_thm := forall LE TE l l' t,
+    I LE TE l t ->
+    L.step LE l l' ->
+    exists t',
+        T.step TE t t' /\
+        I LE TE l' t'.
+
+
+(* program equivalence for Tagged *)
+
+Definition T_rename_globals (rename : nat -> nat) : T.expr -> T.expr :=
+    let fix go e :=
+        let fix go_list es :=
+            match es with
+            | [] => []
+            | e :: es => go e :: go_list es
+            end in
+        let fix go_cases cs :=
+            match cs with
+            | [] => []
+            | (e, r) :: cs => (go e, r) :: go_cases cs
+            end in
+        match e with
+        | T.Arg => T.Arg
+        | T.UpVar i => T.UpVar i
+        | T.Call f a => T.Call (go f) (go a)
+        | T.Constr tag args => T.Constr tag (go_list args)
+        | T.Elim cases target => T.Elim (go_cases cases) (go target)
+        | T.Close fname free => T.Close (rename fname) (go_list free)
+        end in go.
+
+Definition T_rename_globals_list (rename : nat -> nat) :=
+    let go := T_rename_globals rename in
+    let fix go_list es :=
+        match es with
+        | [] => []
+        | e :: es => go e :: go_list es
+        end in go_list.
+
+Definition T_rename_globals_cases (rename : nat -> nat) :=
+    let go := T_rename_globals rename in
+    let fix go_cases cs : list (T.expr * T.rec_info) :=
+        match cs with
+        | [] => []
+        | (e, r) :: cs => (go e, r) :: go_cases cs
+        end in go_cases.
+
+Inductive T_prog_equiv (E1 E2 : T.env) : (nat -> nat) -> T.expr -> T.expr -> Prop :=
+| TProgEquiv : forall rename e1 e2,
+        (forall fname code,
+            nth_error E1 fname = Some code ->
+            (* Looking up the renamed fname gives the renamed function *)
+            nth_error E2 (rename fname) = Some (T_rename_globals rename code)) ->
+        T_rename_globals rename e1 = e2 ->
+        T_prog_equiv E1 E2 rename e1 e2.
+
+
+(* proofs *)
+
+Ltac inject_some := repeat on (Some _ = Some _), invc.
+Ltac break_bind_option :=
+    unfold seq, fmap in *;
+    repeat match goal with
+    | [ H : bind_option ?x _ = Some _ |- _ ] =>
+            destruct x eqn:?; [ simpl in H | discriminate H ]
+    end.
+
+Lemma Forall2_I_compile_list : forall LE TE ls ts,
+    Forall2 (I LE TE) ls ts ->
+    compile_list ls = Some ts.
+induction ls; intros0 Hfa; destruct ts; invc Hfa; simpl in *; eauto.
+unfold seq, fmap.
+specialize (IHls ?? **). rewrite IHls. simpl.
+on (I _ _ _ _), invc. rewrite **. simpl.
+reflexivity.
+Qed.
+
+Lemma I_R_value_fwd : forall LE TE l t,
+    L.value l -> T.value t ->
+    compile_list LE = Some TE ->
+    R LE TE l t -> I LE TE l t.
+induction l using L.expr_ind'; intros0 Lval Tval Henv RR;
+invc Lval; invc RR; invc Tval.
+
+- constructor; eauto.
+  simpl. fold compile_list. unfold seq, fmap.
+
+  assert (forall i,
+    forall l, nth_error args i = Some l ->
+    forall t, nth_error targs i = Some t ->
+    (forall t, L.value l -> T.value t -> compile_list LE = Some TE ->
+        R LE TE l t -> I LE TE l t) ->
+    L.value l -> T.value t ->
+    R LE TE l t ->
+    I LE TE l t) by (intros; eauto).
+  on _, fun H => (assert (Forall2 (I LE TE) args targs) by (list_magic **); clear H).
+  fwd eapply Forall2_I_compile_list as HH; eauto.
+    rewrite HH. clear HH. simpl.
+  reflexivity.
+
+- constructor; eauto.
+  simpl. fold compile_list. unfold seq, fmap.
+
+  assert (forall i,
+    forall l, nth_error free i = Some l ->
+    forall t, nth_error tfree i = Some t ->
+    (forall t, L.value l -> T.value t -> compile_list LE = Some TE ->
+        R LE TE l t -> I LE TE l t) ->
+    L.value l -> T.value t ->
+    R LE TE l t ->
+    I LE TE l t) by (intros; eauto).
+  on _, fun H => (assert (Forall2 (I LE TE) free tfree) by (list_magic **); clear H).
+  fwd eapply Forall2_I_compile_list as HH; eauto.
+    rewrite HH. clear HH. simpl.
+  reflexivity.
+Qed.
+
+
+Lemma compile_list_Forall2 : forall ls ts,
+    compile_list ls = Some ts ->
+    Forall2 (fun l t => compile l = Some t) ls ts.
+induction ls; intros0 Heq; simpl in *; invc Heq.
+- constructor.
+- compute [seq fmap bind_option] in *.
+  destruct (compile _) eqn:?; simpl in *; try discriminate.
+  destruct (compile_list _) eqn:?; simpl in *; try discriminate.
+  on (Some _ = Some _), invc.
+  constructor; eauto.
+Qed.
+
+Lemma compile_list_length : forall es es',
+    compile_list es = Some es' ->
+    length es = length es'.
+intros. eapply Forall2_length. eapply compile_list_Forall2. assumption.
+Qed.
+
+Lemma compile_program_def : forall LE TE l t,
+    compile l = Some t ->
+    compile_list LE = Some TE ->
+    compile_program (l, LE) = Some (t, TE).
+intros0 Heq Heqs.
+unfold compile_program. simpl. rewrite Heq, Heqs. reflexivity.
+Qed.
+
+Ltac inject_pair := repeat on ((_, _) = (_, _)), invc.
+Ltac simpl_compile := simpl in *; fold compile_list in *.
+
+Lemma compile_R : forall LE TE l t,
+    L.value l ->
+    compile_program (l, LE) = Some (t, TE) ->
+    R LE TE l t.
+induction l using L.expr_ind'; intros0 Lval Hcomp;
+invc Lval;
+unfold compile_program in Hcomp.
+
+- break_bind_option. inject_some. inject_pair.
+  simpl_compile. break_bind_option. inject_some.
+  rename l into targs.
+
+  constructor.
+  fwd eapply compile_list_Forall2 with (ls := args); eauto.
+
+  assert (forall i,
+    forall l, nth_error args i = Some l ->
+    forall t, nth_error targs i = Some t ->
+    (forall t, L.value l -> compile_program (l, LE) = Some (t, TE) -> R LE TE l t) ->
+    L.value l ->
+    compile l = Some t ->
+    R LE TE l t) by eauto using compile_program_def.
+  list_magic **.
+
+- break_bind_option. inject_some. inject_pair.
+  simpl_compile. break_bind_option. inject_some.
+  rename l into tfree.
+
+  (* TODO: missing premise: l is well formed, no closures with bad fnames *)
+  assert (exists lbody, nth_error LE f = Some lbody) by admit.  break_exists.
+  fwd eapply length_nth_error_Some with (ys := TE);
+    try eassumption; eauto using compile_list_length.  break_exists.
+  fwd eapply compile_list_Forall2 with (ls := LE); try eassumption.
+  fwd eapply Forall2_nth_error; try eassumption. cbv beta in *.
+
+  econstructor; eauto using compile_program_def.
+
+  fwd eapply compile_list_Forall2 with (ls := free); try eassumption.
+  assert (forall i,
+    forall l, nth_error free i = Some l ->
+    forall t, nth_error tfree i = Some t ->
+    (forall t, L.value l -> compile_program (l, LE) = Some (t, TE) -> R LE TE l t) ->
+    L.value l ->
+    compile l = Some t ->
+    R LE TE l t) by eauto using compile_program_def.
+  list_magic **.
+
+Admitted.
+
+
+Lemma R_value : forall LE TE l t,
+    R LE TE l t ->
+    L.value l ->
+    T.value t.
+induction l using L.expr_ind'; intros0 RR Lval; invc Lval; invc RR; constructor.
+
+- assert (forall i,
+    forall l, nth_error args i = Some l ->
+    forall t, nth_error targs i = Some t ->
+    (forall t, R LE TE l t -> L.value l -> T.value t) ->
+    R LE TE l t ->
+    L.value l ->
+    T.value t) by eauto.
+  list_magic **.
+
+- assert (forall i,
+    forall l, nth_error free i = Some l ->
+    forall t, nth_error tfree i = Some t ->
+    (forall t, R LE TE l t -> L.value l -> T.value t) ->
+    R LE TE l t ->
+    L.value l ->
+    T.value t) by eauto.
+  list_magic **.
+
+Qed.
+
+
+Lemma compile_value : forall l t,
+    compile l = Some t ->
+    L.value l ->
+    T.value t.
+intros.
+fwd eapply compile_R with (LE := []) (TE := []); try eassumption.
+  { unfold compile_program. simpl. unfold seq, fmap. rewrite H. reflexivity. }
+eapply R_value; eauto.
+Qed.
+
+Lemma compile_list_value : forall ls ts,
+    compile_list ls = Some ts ->
+    Forall L.value ls ->
+    Forall T.value ts.
+intros.
+fwd eapply compile_list_Forall2; eauto.
+assert (forall i,
+  forall l, nth_error ls i = Some l ->
+  forall t, nth_error ts i = Some t ->
+  compile l = Some t ->
+  L.value l ->
+  T.value t) by eauto using compile_value.
+list_magic **.
+Qed.
+
+
+Definition T_num_upvars :=
+    let fix go e :=
+        let fix go_list es :=
+            match es with
+            | [] => 0
+            | e :: es => max (go e) (go_list es)
+            end in
+        let fix go_pair p :=
+            match p with
+            | (e, _) => go e
+            end in
+        let fix go_list_pair ps :=
+            match ps with
+            | [] => 0
+            | p :: ps => max (go_pair p) (go_list_pair ps)
+            end in
+        match e with
+        | T.Arg => 0
+        | T.UpVar i => S i
+        | T.Call f a => max (go f) (go a)
+        | T.Constr _ args => go_list args
+        | T.Elim cases target => max (go_list_pair cases) (go target)
+        | T.Close _ free => go_list free
+        end in go.
+
+Definition T_num_upvars_list :=
+    let go := T_num_upvars in
+    let fix go_list es :=
+        match es with
+        | [] => 0
+        | e :: es => max (go e) (go_list es)
+        end in go_list.
+
+Definition T_num_upvars_pair :=
+    let go := T_num_upvars in
+    let fix go_pair (p : T.expr * T.rec_info) :=
+        match p with
+        | (e, _) => go e
+        end in go_pair.
+
+Definition T_num_upvars_list_pair :=
+    let go_pair := T_num_upvars_pair in
+    let fix go_list_pair ps :=
+        match ps with
+        | [] => 0
+        | p :: ps => max (go_pair p) (go_list_pair ps)
+        end in go_list_pair.
+
+Ltac refold_T_num_upvars :=
+    fold T_num_upvars_list in *;
+    fold T_num_upvars_pair in *;
+    fold T_num_upvars_list_pair in *.
+
+
+Ltac T_refold_subst arg vals :=
+    fold (T.subst_list arg vals) in *;
+    fold (T.subst_pair arg vals) in *;
+    fold (T.subst_list_pair arg vals) in *.
+
+Lemma nat_max_le : forall n1 n2 m,
+    max n1 n2 <= m ->
+    n1 <= m /\ n2 <= m.
+intros0 Hle. destruct (Max.max_spec n1 n2) as [[? ?] | [? ?]]; split; omega.
+Qed.
+
+Lemma nat_max_le1 : forall n1 n2 m, max n1 n2 <= m -> n1 <= m.
+intros. destruct (nat_max_le ?? ?? ?? **). assumption.
+Qed.
+
+Lemma nat_max_le2 : forall n1 n2 m, max n1 n2 <= m -> n2 <= m.
+intros. destruct (nat_max_le ?? ?? ?? **). assumption.
+Qed.
+
+Lemma T_Forall_subst_list_exists : forall arg free es,
+    Forall (fun e => exists e', T.subst arg free e = Some e') es ->
+    exists es', T.subst_list arg free es = Some es'.
+induction es; intros0 Hfa; invc Hfa; simpl in *.
+{ eauto. }
+break_exists. find_rewrite.
+specialize (IHes **). break_exists. find_rewrite.
+unfold seq, fmap. simpl. eauto.
+Qed.
+
+Lemma T_num_upvars_list_le_Forall : forall es n,
+    T_num_upvars_list es <= n ->
+    Forall (fun e => T_num_upvars e <= n) es.
+induction es; intros0 Hle; simpl in *.
+{ constructor. }
+destruct (nat_max_le ?? ?? ?? **).
+specialize (IHes ?? **).
+constructor; eauto.
+Qed.
+
+Lemma T_Forall_subst_list_pair_exists : forall arg free es,
+    Forall (fun e => exists e', T.subst_pair arg free e = Some e') es ->
+    exists es', T.subst_list_pair arg free es = Some es'.
+(* copy-pasted from non-pair version above *)
+induction es; intros0 Hfa; invc Hfa; simpl in *.
+{ eauto. }
+break_exists. find_rewrite.
+specialize (IHes **). break_exists. find_rewrite.
+unfold seq, fmap. simpl. eauto.
+Qed.
+
+Lemma T_num_upvars_list_pair_le_Forall : forall es n,
+    T_num_upvars_list_pair es <= n ->
+    Forall (fun e => T_num_upvars_pair e <= n) es.
+(* copy-pasted from non-pair version above *)
+induction es; intros0 Hle; simpl in *.
+{ constructor. }
+destruct (nat_max_le ?? ?? ?? **).
+specialize (IHes ?? **).
+constructor; eauto.
+Qed.
+
+
+Lemma T_num_upvars_subst : forall arg free body,
+    T_num_upvars body <= length free ->
+    exists body', T.subst arg free body = Some body'.
+induction body using T.expr_ind''; intros0 Hup;
+simpl in *; refold_T_num_upvars; T_refold_subst arg free.
+
+- eauto.
+
+- destruct (nth_error _ _) eqn:?; cycle 1.
+    { (* None *) rewrite nth_error_None in *. omega. }
+  eauto.
+
+- unfold seq, fmap.
+  destruct (nat_max_le ?? ?? ?? **).
+  specialize (IHbody1 **). destruct IHbody1 as [? HH1]. rewrite HH1.
+  specialize (IHbody2 **). destruct IHbody2 as [? HH2]. rewrite HH2.
+  simpl. eauto.
+
+- fwd eapply T_num_upvars_list_le_Forall; eauto.
+  fwd eapply T_Forall_subst_list_exists with (es := args).
+    { assert (forall i,
+        forall e, nth_error args i = Some e ->
+        (T_num_upvars e <= length free -> exists e', T.subst arg free e = Some e') ->
+        T_num_upvars e <= length free ->
+        exists e', T.subst arg free e = Some e') by eauto.
+      list_magic **. }
+  break_exists. find_rewrite. unfold seq, fmap. simpl. eauto.
+
+- destruct (nat_max_le _ _ _ **).
+
+  (* cases *)
+  fwd eapply T_num_upvars_list_pair_le_Forall; eauto.
+  fwd eapply T_Forall_subst_list_pair_exists with (es := cases).
+    { assert (forall i,
+        forall p, nth_error cases i = Some p ->
+        (T_num_upvars (fst p) <= length free -> exists e', T.subst arg free (fst p) = Some e') ->
+        T_num_upvars_pair p <= length free ->
+        exists p', T.subst_pair arg free p = Some p'); [ | list_magic ** ].
+      intros. destruct p. simpl in *.
+      fwd refine (_ _); try eassumption. break_exists. repeat find_rewrite.
+      simpl. eauto. }
+  break_exists. find_rewrite.
+
+  (* target *)
+  destruct (IHbody **). repeat find_rewrite.
+
+  unfold seq, fmap. simpl. eauto.
+
+- fwd eapply T_num_upvars_list_le_Forall; eauto.
+  fwd eapply T_Forall_subst_list_exists with (es := free0).
+    { assert (forall i,
+        forall e, nth_error free0 i = Some e ->
+        (T_num_upvars e <= length free -> exists e', T.subst arg free e = Some e') ->
+        T_num_upvars e <= length free ->
+        exists e', T.subst arg free e = Some e') by eauto.
+      list_magic **. }
+  break_exists. find_rewrite. unfold seq, fmap. simpl. eauto.
+
+Qed.
+
+
+
+Definition L_num_upvars :=
+    let fix go e :=
+        let fix go_list es :=
+            match es with
+            | [] => 0
+            | e :: es => max (go e) (go_list es)
+            end in
+        match e with
+        | L.Arg => 0
+        | L.UpVar i => S i
+        | L.Call f a => max (go f) (go a)
+        | L.Constr _ args => go_list args
+        | L.Elim _ cases target => max (go_list cases) (go target)
+        | L.Close _ free => go_list free
+        end in go.
+
+Definition L_num_upvars_list :=
+    let go := L_num_upvars in
+    let fix go_list es :=
+        match es with
+        | [] => 0
+        | e :: es => max (go e) (go_list es)
+        end in go_list.
+
+Ltac refold_L_num_upvars :=
+    fold L_num_upvars_list in *.
+
+Ltac L_refold_subst arg vals :=
+    fold (L.subst_list arg vals) in *.
+
+
+Lemma nat_le_max : forall n1 n2 m,
+    n1 <= m ->
+    n2 <= m ->
+    max n1 n2 <= m.
+intros0 Hle1 Hle2. destruct (Max.max_spec n1 n2) as [[? ?] | [? ?]]; omega.
+Qed.
+
+Lemma L_subst_list_Forall2 : forall arg free es es',
+    L.subst_list arg free es = Some es' ->
+    Forall2 (fun e e' => L.subst arg free e = Some e') es es'.
+induction es; intros0 Hsub; destruct es'.
+- constructor.
+- simpl in Hsub. discriminate.
+- simpl in Hsub. break_bind_option. inject_some. discriminate.
+- simpl in Hsub. break_bind_option. inject_some.
+  on (_ :: _ = _ :: _), invc.
+  constructor; eauto.
+Qed.
+
+Lemma L_Forall_num_upvars_list_le : forall es n,
+    Forall (fun e => L_num_upvars e <= n) es ->
+    L_num_upvars_list es <= n.
+induction es; intros0 Hle; simpl in *.
+{ omega. }
+invc Hle.  eapply nat_le_max; eauto.
+Qed.
+
+Lemma L_subst_num_upvars : forall arg free body body',
+    L.subst arg free body = Some body' ->
+    L_num_upvars body <= length free.
+induction body using L.expr_ind'; intros0 Hsub;
+simpl in *; refold_L_num_upvars; L_refold_subst arg free.
+
+- omega.
+
+- assert (HH : nth_error free n <> None) by congruence.
+  rewrite nth_error_Some in HH.
+  omega.
+
+- break_bind_option. inject_some.
+  specialize (IHbody1 ?? ***).
+  specialize (IHbody2 ?? ***).
+  eauto using nat_le_max.
+
+- break_bind_option. inject_some.
+  fwd eapply L_subst_list_Forall2; try eassumption.
+  rename l into args'.
+  eapply L_Forall_num_upvars_list_le.
+  assert (forall i,
+    forall e, nth_error args i = Some e ->
+    forall e', nth_error args' i = Some e' ->
+    (forall e', L.subst arg free e = Some e' -> L_num_upvars e <= length free) ->
+    L.subst arg free e = Some e' ->
+    L_num_upvars e <= length free) by eauto.
+  list_magic **.
+
+- break_bind_option. inject_some.
+
+  (* target *)
+  specialize (IHbody _ ***). eapply nat_le_max; eauto.
+
+  (* cases *)
+  fwd eapply L_subst_list_Forall2; eauto.
+  rename l into cases'.
+  eapply L_Forall_num_upvars_list_le.
+  assert (forall i,
+    forall e, nth_error cases i = Some e ->
+    forall e', nth_error cases' i = Some e' ->
+    (forall e', L.subst arg free e = Some e' -> L_num_upvars e <= length free) ->
+    L.subst arg free e = Some e' ->
+    L_num_upvars e <= length free) by eauto.
+  list_magic **.
+
+- break_bind_option. inject_some.
+  fwd eapply L_subst_list_Forall2; try eassumption.
+  rename free0 into es.
+  rename l into es'.
+  eapply L_Forall_num_upvars_list_le.
+  assert (forall i,
+    forall e, nth_error es i = Some e ->
+    forall e', nth_error es' i = Some e' ->
+    (forall e', L.subst arg free e = Some e' -> L_num_upvars e <= length free) ->
+    L.subst arg free e = Some e' ->
+    L_num_upvars e <= length free) by eauto.
+  list_magic **.
+
+Qed.
+
+
+Lemma compile_num_upvars : forall l t,
+    compile l = Some t ->
+    L_num_upvars l = T_num_upvars t.
+induction l using L.expr_ind'; intros0 Hcomp;
+simpl_compile; refold_L_num_upvars.
+
+- inject_some. simpl. reflexivity.
+
+- inject_some. simpl. reflexivity.
+
+- break_bind_option. inject_some.
+  specialize (IHl1 _ ***). find_rewrite.
+  specialize (IHl2 _ ***). find_rewrite.
+  simpl. reflexivity.
+
+- break_bind_option. inject_some. simpl. refold_T_num_upvars.
+  admit.
+
+- admit.
+
+- admit.
+Admitted.
+
+
+Theorem I_sim : forall LE TE l l' t,
+    I LE TE l t ->
+    L.step LE l l' ->
+    exists t',
+        T.step TE t t' /\
+        I LE TE l' t'.
+induction l using L.expr_ind'; intros0 II Lstep;
+invc Lstep; invc II; simpl_compile; break_bind_option; inject_some.
+
+- (* MakeCall *)
+  fwd eapply length_nth_error_Some with (ys := TE); try eassumption.
+    { eauto using compile_list_length. }
+  break_exists.
+
+  fwd eapply compile_list_Forall2 with (ls := LE) (ts := TE); eauto.
+  fwd eapply Forall2_nth_error; eauto. cbv beta in *.
+
+  rename l into tfree.
+  rename e1 into t2.
+  rename x into te.
+  fwd eapply T_num_upvars_subst with (arg := t2) (free := tfree) (body := te).
+    { erewrite <- compile_num_upvars by eauto.
+      erewrite <- compile_list_length by eauto.
+      eapply L_subst_num_upvars; eauto. }
+  break_exists.
+
+  eexists. split. eapply T.MakeCall; eauto.
+  + eauto using compile_value.
+  + eauto using compile_list_value.
+  + admit. (* subst preserves I *)
+
+- admit.
+- admit.
+- admit.
+- admit.
+- admit.
+- admit.
+
+Admitted.
